- To solve this question we implement the **recurrence relation**. The tribonacci sequence is defined as 
	- T(0) = 0 
	- T(1) = 1
	- T(2) = 1
	- T(n+3) = T(n) + T(n+1) + T(n+2) for n â‰¥ 0. 
- To solve this we work backwards for a solution: 
	- Where T = T(n-1) + T(n-2) + T(n-3)
- A solution for this would look like: 

```python
class Solution 
	def tribonacci(self, n:int): 
		if n == 0: 
			return 0
		else n == 1 or n == 2: 
			return 1
		return self.tribonacci(n-1) + self.tribonacci(n-2) + self.tribonacci(n-3)
```

- This solution works for smaller numbers, however, for larger values we will hit a **TLE error**
- To get around this we use a dynamic programming approach: 

```python
class Solution:
	def tribonacci(self, n: int) -> int:
		if n == 0:
			return 0
		elif n == 1 or n == 2:
			return 1

		t0, t1, t2 = 0, 1, 1
		for _ in range(3, n+1):
			t3 = t0 + t1+ t2
			t0, t1, t2 = t1, t2, t3

		return t2
```

- This approach uses **iterative dynamic programming** basically we set the first 3 values and then iterate through getting t3 by adding the three values and then shifting the values up to replace t0, t1, and t2
